doot

_notes/Languages/lean/myproject/IMP.lean
@@ -6,7 +6,7 @@
 -- Local Open Scope list_scope.
 
 -- import home.philip.Documents.lean.std4.Std.Data.Int.Basics
-import std.Std.Data.List.Basic
+import Std.Data.List.Basic
 
 #eval Lean.versionString
 #eval 1 + 1
@@ -14,9 +14,9 @@ import std.Std.Data.List.Basic
 #check "string"
 
 /-
--- (** * 1. The source language: IMP *)
+-- /-* * 1. The source language: IMP -/
 -/
--- (** ** 1.1 Arithmetic expressions *)
+-- /-* ** 1.1 Arithmetic expressions -/
 
 
 def ident : Type := String
@@ -24,21 +24,21 @@ def ident : Type := String
 -- def mythree : Nat := 3
 -- type ident = string
 
--- (** The abstract syntax: an arithmetic expression is either... *)
+-- /-* The abstract syntax: an arithmetic expression is either... -/
 def myid : forall {a :Type}, a -> a := fun x => x
 def myid2 : {a :Type} -> a -> a := fun x => x
 #check myid
 
 inductive aexp where
-  | CONST (n : Int) : aexp --                      (**r a constant, or *)
-  | VAR (x : ident) : aexp --                   (**r a variable, or *)
-  | PLUS (a1 : aexp) (a2 : aexp) : aexp --        (**r a sum of two expressions, or *)
-  | MINUS (a1 : aexp) (a2 : aexp) : aexp --      (**r a difference of two expressions *)
+  | CONST (n : Int) : aexp --                      /-*r a constant, or -/
+  | VAR (x : ident) : aexp --                   /-*r a variable, or -/
+  | PLUS (a1 : aexp) (a2 : aexp) : aexp --        /-*r a sum of two expressions, or -/
+  | MINUS (a1 : aexp) (a2 : aexp) : aexp --      /-*r a difference of two expressions -/
 
 
-/-(** The denotational semantics: an evaluation function that computes
+/- /- * The denotational semantics: an evaluation function that computes
   the integer value denoted by an expression.  It is parameterized by
-  a store [s] that associates values to variables. *)
+  a store [s] that associates values to variables. -/
 -/
 
 
@@ -52,21 +52,25 @@ def aeval (s: store) (a: aexp) : Int :=
   | aexp.MINUS a1 a2 => aeval s a1 - aeval s a2
 
 
---(** Such evaluation functions / denotational semantics have many uses.
---    First, we can use [aeval] to evaluate a given expression in a given store. *)
+--/-* Such evaluation functions / denotational semantics have many uses.
+--    First, we can use [aeval] to evaluate a given expression in a given store. -/
 
 #eval (aeval (fun _x => 2) (aexp.PLUS (aexp.VAR "x") (aexp.MINUS (aexp.VAR "x") (aexp.CONST 1))))
 
--- (** Result is: [ = 3 : Z ]. *)
 
--- (** We can also do partial evaluation with respect to an unknown store *)
+-- /-* Result is: [ = 3 : Z ]. -/
+
+-- /-* We can also do partial evaluation with respect to an unknown store -/
 open aexp
--- #eval (fun s => aeval s (PLUS (VAR "x") (MINUS (CONST 10) (CONST 1))))
+-- hmm #eval doesn't work. #reduce is a little too aggressive
+#reduce (fun s => aeval s (PLUS (VAR "x") (MINUS (CONST 10) (CONST 1))))
+-- example : forall s, 42 =  aeval s (PLUS (VAR "x") (MINUS (CONST 10) (CONST 1))) := by
+--  intros
+--  simp [aeval]
 
+--/-* Result is: [ = fun s : store => s "x" + 9 ]. -/
 
---(** Result is: [ = fun s : store => s "x" + 9 ]. *)
-
--- (** We can prove properties of a given expression. *)
+-- /-* We can prove properties of a given expression. -/
 
 
 theorem aeval_xplus1 :
@@ -85,42 +89,54 @@ Proof.
 Qed.
 -/
 /-
-(** Finally, we can prove "meta-properties" that hold for all expressions.
+/-* Finally, we can prove "meta-properties" that hold for all expressions.
   For example: the value of an expression depends only on the values of its
   free variables.
 
   Free variables are defined by this recursive predicate:
-*)
-
-Fixpoint free_in_aexp (x: ident) (a: aexp) : Prop :=
+-/
+-/
+def free_in_aexp (x: ident) (a: aexp) : Prop :=
   match a with
   | CONST n => False
   | VAR y => y = x
   | PLUS a1 a2 | MINUS a1 a2 => free_in_aexp x a1 \/ free_in_aexp x a2
-  end.
 
-Theorem aeval_free:
+
+
+theorem aeval_free:
   forall s1 s2 a,
   (forall x, free_in_aexp x a -> s1 x = s2 x) ->
-  aeval s1 a = aeval s2 a.
+  aeval s1 a = aeval s2 a := by
+  intros s1 s2 a
+  induction a <;> simp [aeval] <;> intros hyp
+  -- case CONST n => simp [aeval]
+  case VAR x => apply hyp; simp [free_in_aexp]
+  -- what a mess
+  case PLUS a1 a2 => rw [a1, a2] <;> intros x f <;> apply hyp <;> simp [free_in_aexp]; apply Or.inr; assumption; apply Or.inl; assumption
+  case MINUS a1 a2 => rw [a1, a2] <;> intros x f <;> apply hyp <;> simp [free_in_aexp]; apply Or.inr; assumption; apply Or.inl; assumption
+
+
+#check "hello"
+/-
 Proof.
   induction a; cbn; intros SAMEFREE.
-- (* Case a = CONST n *)
+- /- Case a = CONST n -/
   auto.
-- (* Case a = VAR x *)
+- /- Case a = VAR x -/
   apply SAMEFREE. auto.
-- (* Case a = PLUS a1 a2 *)
+- /- Case a = PLUS a1 a2 -/
   rewrite IHa1, IHa2. auto. auto. auto.
-- (* Case a = MINUS a1 a2 *)
+- /- Case a = MINUS a1 a2 -/
   rewrite IHa1, IHa2; auto.
 Qed.
 
-(** *** Exercise (1 star, recommended). *)
-(** Add support for multiplication in arithmetic expressions.
-  Modify the [aexp] type and the [aeval] function accordingly. *)
+/-* *** Exercise (1 star, recommended). -/
+/-* Add support for multiplication in arithmetic expressions.
+  Modify the [aexp] type and the [aeval] function accordingly. -/
 
-(** *** Exercise (2 stars, recommended). *)
-(** Add support for division and for detecting arithmetic overflow.
+/-* *** Exercise (2 stars, recommended). -/
+/-* Add support for division and for detecting arithmetic overflow.
   With this extension, the evaluation of an expression can produce an
   error: integer division by zero or result that exceeds the range
   [[min_int, max_int]].  You can either change the type of the
@@ -135,82 +151,89 @@ Qed.
   Inductive aeval_rel: store -> aexp -> Z -> Prop := ...
 >>
   Some definitions you can use:
-*)
+-/
+-/
 
-Definition min_int := - (2 ^ 63).
-Definition max_int := 2 ^ 63 - 1.
-Definition check_for_overflow (n: Z): option Z :=
-  if n <? min_int then None else if n >? max_int then None else Some n.
+#check Int.pow
+def min_int := - ((2 : Int) ^ 63)
+def max_int := (2 : Int) ^ 63 - 1
+def check_for_overflow (n: Int): Option Int :=
+  if n < min_int then none else if n > max_int then none else some n
 
-(** ** 1.3 Boolean expressions *)
+#eval (check_for_overflow 2222222222222222222)
 
-(** The IMP language has conditional statements (if/then/else) and
+/-
+/-* ** 1.3 Boolean expressions -/
+
+/-* The IMP language has conditional statements (if/then/else) and
   loops.  They are controlled by expressions that evaluate to Boolean
-  values.  Here is the abstract syntax of Boolean expressions. *)
+  values.  Here is the abstract syntax of Boolean expressions. -/
 
-Inductive bexp : Type :=
-  | TRUE                              (**r always true *)
-  | FALSE                             (**r always false *)
-  | EQUAL (a1: aexp) (a2: aexp)       (**r whether [a1 = a2] *)
-  | LESSEQUAL (a1: aexp) (a2: aexp)   (**r whether [a1 <= a2] *)
-  | NOT (b1: bexp)                    (**r Boolean negation *)
-  | AND (b1: bexp) (b2: bexp).        (**r Boolean conjunction *)
-
-(** Just like arithmetic expressions evaluate to integers,
-  Boolean expressions evaluate to Boolean values [true] or [false]. *)
-
-Fixpoint beval (s: store) (b: bexp) : bool :=
+-/
+inductive bexp : Type :=
+  | TRUE                         --     /-*r always true -/
+  | FALSE                          --   /-*r always false -/
+  | EQUAL (a1: aexp) (a2: aexp)     --  /-*r whether [a1 = a2] -/
+  | LESSEQUAL (a1: aexp) (a2: aexp) --  /-*r whether [a1 <= a2] -/
+  | NOT (b1: bexp)                  --  /-*r Boolean negation -/
+  | AND (b1: bexp) (b2: bexp)      --  /-*r Boolean conjunction -/
+/-
+/-* Just like arithmetic expressions evaluate to integers,
+  Boolean expressions evaluate to Boolean values [true] or [false]. -/
+-/
+open bexp
+def beval (s: store) (b: bexp) : Bool :=
   match b with
   | TRUE => true
   | FALSE => false
-  | EQUAL a1 a2 => aeval s a1 =? aeval s a2
-  | LESSEQUAL a1 a2 => aeval s a1 <=? aeval s a2
-  | NOT b1 => negb (beval s b1)
+  | EQUAL a1 a2 => aeval s a1 == aeval s a2
+  | LESSEQUAL a1 a2 => aeval s a1 <= aeval s a2
+  | NOT b1 => not (beval s b1)
   | AND b1 b2 => beval s b1 && beval s b2
-  end.
 
-(** There are many useful derived forms. *)
+-- /-* There are many useful derived forms. -/
 
-Definition NOTEQUAL (a1 a2: aexp) : bexp := NOT (EQUAL a1 a2).
+def NOTEQUAL (a1 a2: aexp) : bexp := NOT (EQUAL a1 a2)
 
-Definition GREATEREQUAL (a1 a2: aexp) : bexp := LESSEQUAL a2 a1.
+def GREATEREQUAL (a1 a2: aexp) : bexp := LESSEQUAL a2 a1
 
-Definition GREATER (a1 a2: aexp) : bexp := NOT (LESSEQUAL a1 a2).
+def GREATER (a1 a2: aexp) : bexp := NOT (LESSEQUAL a1 a2)
 
-Definition LESS (a1 a2: aexp) : bexp := GREATER a2 a1.
+def LESS (a1 a2: aexp) : bexp := GREATER a2 a1
 
-Definition OR (b1 b2: bexp) : bexp := NOT (AND (NOT b1) (NOT b2)).
+def OR (b1 b2: bexp) : bexp := NOT (AND (NOT b1) (NOT b2))
 
-(** *** Exercise (1 star, recommended) *)
-(** Show the expected semantics for the [OR] derived form: *)
+-- /- * *** Exercise (1 star, recommended) -/
+-- /- * Show the expected semantics for the [OR] derived form: -/
 
-Lemma beval_OR:
-  forall s b1 b2, beval s (OR b1 b2) = beval s b1 || beval s b2.
+lemma beval_OR :
+  forall s b1 b2, beval s (OR b1 b2) = beval s b1 || beval s b2 := by
+/-
 Proof.
   intros; cbn.
-  (* Hint: do "SearchAbout negb" to see the available lemmas about Boolean negation. *)
-  (* Hint: or just do a case analysis on [beval s b1] and [beval s b2], there are
-     only 4 cases to consider. *)
-  (* FILL IN HERE *)
+  /- Hint: do "SearchAbout negb" to see the available lemmas about Boolean negation. -/
+  /- Hint: or just do a case analysis on [beval s b1] and [beval s b2], there are
+     only 4 cases to consider. -/
+  /- FILL IN HERE -/
 Abort.
+-/
+/-* ** 1.4 Commands -/
 
-(** ** 1.4 Commands *)
-
-(** To complete the definition of the IMP language, here is the
-  abstract syntax of commands, also known as statements. *)
+/-* To complete the definition of the IMP language, here is the
+  abstract syntax of commands, also known as statements. -/
 
 Inductive com: Type :=
-  | SKIP                                     (**r do nothing *)
-  | ASSIGN (x: ident) (a: aexp)              (**r assignment: [v := a] *)
-  | SEQ (c1: com) (c2: com)                  (**r sequence: [c1; c2] *)
-  | IFTHENELSE (b: bexp) (c1: com) (c2: com) (**r conditional: [if b then c1 else c2] *)
-  | WHILE (b: bexp) (c1: com).               (**r loop: [while b do c1 done] *)
+  | SKIP                                     /-*r do nothing -/
+  | ASSIGN (x: ident) (a: aexp)              /-*r assignment: [v := a] -/
+  | SEQ (c1: com) (c2: com)                  /-*r sequence: [c1; c2] -/
+  | IFTHENELSE (b: bexp) (c1: com) (c2: com) /-*r conditional: [if b then c1 else c2] -/
+  | WHILE (b: bexp) (c1: com).               /-*r loop: [while b do c1 done] -/
 
-(** We can write [c1 ;; c2] instead of [SEQ c1 c2], it is easier on the eyes. *)
+/-* We can write [c1 ;; c2] instead of [SEQ c1 c2], it is easier on the eyes. -/
 
 Infix ";;" := SEQ (at level 80, right associativity).
 
-(** Here is an IMP program that performs Euclidean division by
+/-* Here is an IMP program that performs Euclidean division by
   repeated subtraction.  At the end of the program, "q" contains
   the quotient of "a" by "b", and "r" contains the remainder.
   In pseudocode:
@@ -219,27 +242,27 @@ Infix ";;" := SEQ (at level 80, right associativity).
        while b <= r do r := r - b; q := q + 1 done
 >>
   In abstract syntax:
-*)
+-/
 
-Definition Euclidean_division :=
+def Euclidean_division :=
   ASSIGN "r" (VAR "a") ;;
   ASSIGN "q" (CONST 0) ;;
   WHILE (LESSEQUAL (VAR "b") (VAR "r"))
     (ASSIGN "r" (MINUS (VAR "r") (VAR "b")) ;;
      ASSIGN "q" (PLUS (VAR "q") (CONST 1))).
 
-(** A useful operation over stores:
+/-* A useful operation over stores:
     [update x v s] is the store that maps [x] to [v] and is equal to [s] for
-    all variables other than [x]. *)
+    all variables other than [x]. -/
 
-Definition update (x: ident) (v: Z) (s: store) : store :=
+def update (x: ident) (v: Z) (s: store) : store :=
   fun y => if string_dec x y then v else s y.
 
-(** A naive approach to giving semantics to commands is to write an
+/-* A naive approach to giving semantics to commands is to write an
   evaluation function [cexec s c] that runs the command [c] in initial
-  store [s] and returns the final store when [c] terminates. *)
+  store [s] and returns the final store when [c] terminates. -/
 
-Fail Fixpoint cexec (s: store) (c: com) : store :=
+Fail def cexec (s: store) (c: com) : store :=
   match c with
   | SKIP => s
   | ASSIGN x a => update x (aeval s a) s
@@ -249,9 +272,9 @@ Fail Fixpoint cexec (s: store) (c: com) : store :=
       if beval s b
       then (let s' := cexec s c1 in cexec s' (WHILE b c1))
       else s
-  end.
+  
 
-(** The definition above is rejected by Coq, and rightly so, because
+/-* The definition above is rejected by Coq, and rightly so, because
   all Coq functions must terminate, yet the [WHILE] case may not
   terminate.  Consider for example the infinite loop [WHILE TRUE
   SKIP].
@@ -265,7 +288,7 @@ Fail Fixpoint cexec (s: store) (c: com) : store :=
   [cexec s c s'] that holds iff command [c], started in state [s],
   terminates with state [s'].  This relation can easily be defined as
   a Coq inductive predicate:
-*)
+-/
 
 Inductive cexec: store -> com -> store -> Prop :=
   | cexec_skip: forall s,
@@ -285,16 +308,16 @@ Inductive cexec: store -> com -> store -> Prop :=
       beval s b = true -> cexec s c s' -> cexec s' (WHILE b c) s'' ->
       cexec s (WHILE b c) s''.
 
-(** This style of semantics is known as natural semantics or big-step
+/-* This style of semantics is known as natural semantics or big-step
   operational semantics.  The predicate [cexec s c s'] holds iff there
   exists a finite derivation of this conclusion, using the axioms and
   inference rules above.  The structure of the derivation represents
   the computations performed by [c] in a tree-like manner.  The
   finiteness of the derivation guarantees that only terminating
   executions satisfy [cexec].  Indeed, [WHILE TRUE SKIP] does not
-  satisfy [cexec]: *)
+  satisfy [cexec]: -/
 
-Lemma cexec_infinite_loop:
+lemma cexec_infinite_loop:
   forall s, ~ exists s', cexec s (WHILE TRUE SKIP) s'.
 Proof.
   assert (A: forall s c s', cexec s c s' -> c = WHILE TRUE SKIP -> False).
@@ -305,13 +328,13 @@ Proof.
   intros s (s' & EXEC). apply A with (s := s) (c := WHILE TRUE SKIP) (s' := s'); auto.
 Qed.
 
-(** Our naive idea of an execution function for commands was not
+/-* Our naive idea of an execution function for commands was not
   completely off.  We can define an approximation of such a function
   by bounding a priori the recursion depth, using a [fuel] parameter
   of type [nat].  When the fuel drops to 0, [None] is returned,
-  meaning that the final store could not be computed. *)
+  meaning that the final store could not be computed. -/
 
-Fixpoint cexec_bounded (fuel: nat) (s: store) (c: com) : option store :=
+def cexec_bounded (fuel: nat) (s: store) (c: com) : option store :=
   match fuel with
   | O => None
   | S fuel' =>
@@ -322,7 +345,7 @@ Fixpoint cexec_bounded (fuel: nat) (s: store) (c: com) : option store :=
           match cexec_bounded fuel' s c1 with
           | None  => None
           | Some s' => cexec_bounded fuel' s' c2
-          end
+          
       | IFTHENELSE b c1 c2 =>
           if beval s b then cexec_bounded fuel' s c1 else cexec_bounded fuel' s c2
       | WHILE b c1 =>
@@ -330,53 +353,53 @@ Fixpoint cexec_bounded (fuel: nat) (s: store) (c: com) : option store :=
             match cexec_bounded fuel' s c1 with
             | None  => None
             | Some s' => cexec_bounded fuel' s' (WHILE b c1)
-            end
+            
           else Some s
-      end
-  end.
+      
+  
 
-(** This bounded execution function is great for testing programs.
+/-* This bounded execution function is great for testing programs.
     For example, let's compute the quotient and the remainder of 14 by
-    3 using the Euclidean division program above. *)
+    3 using the Euclidean division program above. -/
 
 Eval compute in
   (let s := update "a" 14 (update "b" 3 (fun _ => 0)) in
    match cexec_bounded 100 s Euclidean_division with
    | None => None
    | Some s' => Some (s' "q", s' "r")
-   end).
+   ).
 
-(** *** Exercise (3 stars, optional) *)
-(** Relate the [cexec] relation with the [cexec_bounded] function by
-  proving the following two lemmas. *)
+/-* *** Exercise (3 stars, optional) -/
+/-* Relate the [cexec] relation with the [cexec_bounded] function by
+  proving the following two lemmas. -/
 
-Lemma cexec_bounded_sound:
+lemma cexec_bounded_sound:
   forall fuel s c s', cexec_bounded fuel s c = Some s' -> cexec s c s'.
 Proof.
   induction fuel as [ | fuel ]; cbn; intros.
 - discriminate.
 - destruct c.
-  (* FILL IN HERE *)
+  /- FILL IN HERE -/
 Abort.
 
-Lemma cexec_bounded_complete:
+lemma cexec_bounded_complete:
   forall s c s', cexec s c s' ->
   exists fuel1, forall fuel, (fuel >= fuel1)%nat -> cexec_bounded fuel s c = Some s'.
 Proof.
   induction 1.
-  (* FILL IN HERE *)
+  /- FILL IN HERE -/
 Abort.
 
-(** * 6. Small-step semantics for IMP *)
+/-* * 6. Small-step semantics for IMP -/
 
-(** * 6.1 Reduction semantics *)
+/-* * 6.1 Reduction semantics -/
 
-(** In small-step style, the semantics is presented as a one-step
+/-* In small-step style, the semantics is presented as a one-step
   reduction relation [ red (c, s) (c', s') ], meaning that the command
   [c], executed in initial state [s], performs one elementary step of
   computation.  [s'] is the updated state after this step.  [c'] is
   the residual command, capturing all the computations that remain to
-  be done.  *)
+  be done.  -/
 
 Inductive red: com * store -> com * store -> Prop :=
   | red_assign: forall x a s,
@@ -395,32 +418,32 @@ Inductive red: com * store -> com * store -> Prop :=
       beval s b = true ->
       red (WHILE b c, s) (SEQ c (WHILE b c), s).
 
-(** *** Exercise (2 stars, recommended) *)
-(** Show that Imp programs cannot go wrong.  Hint: first prove the following
-  "progress" result for non-[SKIP] commands. *)
+/-* *** Exercise (2 stars, recommended) -/
+/-* Show that Imp programs cannot go wrong.  Hint: first prove the following
+  "progress" result for non-[SKIP] commands. -/
 
-Lemma red_progress:
+lemma red_progress:
   forall c s, c = SKIP \/ exists c', exists s', red (c, s) (c', s').
 Proof.
   induction c; intros.
-  (* FILL IN HERE *)
+  /- FILL IN HERE -/
 Abort.
 
-Definition goes_wrong (c: com) (s: store) : Prop :=
+def goes_wrong (c: com) (s: store) : Prop :=
   exists c', exists s',
   star red (c, s) (c', s') /\ irred red (c', s') /\ c' <> SKIP.
 
-Lemma not_goes_wrong:
+lemma not_goes_wrong:
   forall c s, ~(goes_wrong c s).
 Proof.
   intros c s (c' & s' & STAR & IRRED & NOTSKIP).
-  (* FILL IN HERE *)
+  /- FILL IN HERE -/
 Abort.
 
-(** Sequences of reductions can go under a sequence context, generalizing
-  rule [red_seq_step]. *)
+/-* Sequences of reductions can go under a sequence context, generalizing
+  rule [red_seq_step]. -/
 
-Lemma red_seq_steps:
+lemma red_seq_steps:
   forall c2 s c s' c',
   star red (c, s) (c', s') -> star red ((c;;c2), s) ((c';;c2), s').
 Proof.
@@ -430,63 +453,63 @@ Proof.
   apply star_step with (c1;;c2, st1). apply red_seq_step. auto. auto.  
 Qed.
 
-(** We now recall the equivalence result between 
+/-* We now recall the equivalence result between 
 - termination according to the big-step semantics
 - existence of a finite sequence of reductions to [SKIP]
   according to the small-step semantics.
 
 We start with the implication big-step ==> small-step, which is
-a straightforward induction on the big-step evaluation derivation. *)
+a straightforward induction on the big-step evaluation derivation. -/
 
 Theorem cexec_to_reds:
   forall s c s', cexec s c s' -> star red (c, s) (SKIP, s').
 Proof.
   induction 1.
-- (* SKIP *)
+- /- SKIP -/
   apply star_refl.
-- (* ASSIGN *)
+- /- ASSIGN -/
   apply star_one. apply red_assign. 
-- (* SEQ *)
+- /- SEQ -/
   eapply star_trans. apply red_seq_steps. apply IHcexec1.
   eapply star_step.  apply red_seq_done.  apply IHcexec2.
-- (* IFTHENELSE *)
+- /- IFTHENELSE -/
   eapply star_step. apply red_ifthenelse. auto.
-- (* WHILE stop *)
+- /- WHILE stop -/
   apply star_one. apply red_while_done. auto.
-- (* WHILE loop *)
+- /- WHILE loop -/
   eapply star_step. apply red_while_loop. auto.
   eapply star_trans. apply red_seq_steps. apply IHcexec1.
   eapply star_step. apply red_seq_done. apply IHcexec2.
 Qed.
 
-(** The reverse implication, from small-step to big-step, is more subtle.
+/-* The reverse implication, from small-step to big-step, is more subtle.
 The key lemma is the following, showing that one step of reduction
 followed by a big-step evaluation to a final state can be collapsed
-into a single big-step evaluation to that final state. *)
+into a single big-step evaluation to that final state. -/
 
-Lemma red_append_cexec:
+lemma red_append_cexec:
   forall c1 s1 c2 s2, red (c1, s1) (c2, s2) ->
   forall s', cexec s2 c2 s' -> cexec s1 c1 s'.
 Proof.
   intros until s2; intros STEP. dependent induction STEP; intros.
-- (* red_assign *)
+- /- red_assign -/
   inversion H; subst. apply cexec_assign. 
-- (* red_seq_done *)
+- /- red_seq_done -/
   apply cexec_seq with s2. apply cexec_skip. auto.
-- (* red seq step *)
+- /- red seq step -/
   inversion H; subst. apply cexec_seq with s'0.
   eapply IHSTEP; eauto.
   auto.
-- (* red_ifthenelse *)
+- /- red_ifthenelse -/
   apply cexec_ifthenelse. auto.
-- (* red_while_done *)
+- /- red_while_done -/
   inversion H0; subst. apply cexec_while_done. auto.
-- (* red while loop *)
+- /- red while loop -/
   inversion H0; subst. apply cexec_while_loop with s'0; auto.
 Qed.
 
-(** As a consequence, a term that reduces to [SKIP] evaluates in big-step
-  with the same final state. *)
+/-* As a consequence, a term that reduces to [SKIP] evaluates in big-step
+  with the same final state. -/
 
 Theorem reds_to_cexec:
   forall s c s',
@@ -497,9 +520,9 @@ Proof.
 - destruct b as [c1 s1]. apply red_append_cexec with c1 s1; auto.
 Qed.
 
-(** ** 6.2 Transition semantics with continuations *)
+/-* ** 6.2 Transition semantics with continuations -/
 
-(** We now introduce an alternate form of small-step semantics
+/-* We now introduce an alternate form of small-step semantics
   where the command to be executed is explicitly decomposed into:
 - a sub-command under focus, where computation takes place;
 - a continuation (or context) describing the position of this sub-command
@@ -512,14 +535,14 @@ continuation, state).  Previously, we had transitions between pairs
 (whole-command, state).
 
 The syntax of continuations is as follows:
-*)
+-/
 
-Inductive cont : Type :=
+inductive cont : Type :=
   | Kstop
   | Kseq (c: com) (k: cont)
   | Kwhile (b: bexp) (c: com) (k: cont).
 
-(** Intuitive meaning of these constructors:
+/-* Intuitive meaning of these constructors:
 - [Kstop] means that, after the sub-command under focus terminates,
   nothing remains to be done, and execution can stop.  In other words,
   the sub-command under focus is the whole command.
@@ -527,22 +550,22 @@ Inductive cont : Type :=
   to execute command [c] in sequence, then continue as described by [k].
 - [Kwhile b c k] means that, after the sub-command terminates, we still need
   to execute a loop [WHILE b DO c END], then continue as described by [k].
-*)
+-/
 
-(** Another way to forge intuitions about continuations is to ponder the following
+/-* Another way to forge intuitions about continuations is to ponder the following
   [apply_cont k c] function, which takes a sub-command [c] under focus
   and a continuation [k], and rebuilds the whole command.  It simply
   puts [c] in lefmost position in a nest of sequences as described by [k].
-*)
+-/
 
-Fixpoint apply_cont (k: cont) (c: com) : com :=
+def apply_cont (k: cont) (c: com) : com :=
   match k with
   | Kstop => c
   | Kseq c1 k1 => apply_cont k1 (SEQ c c1)
   | Kwhile b1 c1 k1 => apply_cont k1 (SEQ c (WHILE b1 c1))
-  end.
+  
 
-(** Transitions between (subcommand-under-focus, continuation, state)
+/-* Transitions between (subcommand-under-focus, continuation, state)
   triples perform conceptually different kinds of actions:
 - Computation: evaluate an arithmetic expression or boolean expression
   and modify the triple according to the result of the evaluation.
@@ -552,37 +575,37 @@ Fixpoint apply_cont (k: cont) (c: com) : com :=
   look at the head of the continuation to see what to do next.
 
 Here are the transition rules, classified by the kinds of actions they implement.
-*)
+-/
 
-Inductive step: com * cont * store -> com * cont * store -> Prop :=
+inductive step: com * cont * store -> com * cont * store -> Prop :=
 
-  | step_assign: forall x a k s,              (**r computation for assignments *)
+  | step_assign: forall x a k s,              /-*r computation for assignments -/
       step (ASSIGN x a, k, s) (SKIP, k, update x (aeval s a) s)
 
-  | step_seq: forall c1 c2 s k,               (**r focusing for sequence *)
+  | step_seq: forall c1 c2 s k,               /-*r focusing for sequence -/
       step (SEQ c1 c2, k, s) (c1, Kseq c2 k, s)
 
-  | step_ifthenelse: forall b c1 c2 k s,      (**r computation for conditionals *)
+  | step_ifthenelse: forall b c1 c2 k s,      /-*r computation for conditionals -/
       step (IFTHENELSE b c1 c2, k, s) ((if beval s b then c1 else c2), k, s)
 
-  | step_while_done: forall b c k s,          (**r computation for loops *)
+  | step_while_done: forall b c k s,          /-*r computation for loops -/
       beval s b = false ->
       step (WHILE b c, k, s) (SKIP, k, s)
 
-  | step_while_true: forall b c k s,          (**r computation and focusSKIing for loops *)
+  | step_while_true: forall b c k s,          /-*r computation and focusSKIing for loops -/
       beval s b = true ->
       step (WHILE b c, k, s) (c, Kwhile b c k, s)
 
-  | step_skip_seq: forall c k s,              (**r resumption *)
+  | step_skip_seq: forall c k s,              /-*r resumption -/
       step (SKIP, Kseq c k, s) (c, k, s)
 
-  | step_skip_while: forall b c k s,          (**r resumption *)
+  | step_skip_while: forall b c k s,          /-*r resumption -/
       step (SKIP, Kwhile b c k, s) (WHILE b c, k, s).
 
 
-(** *** Extensions to other control structures *)
+/-* *** Extensions to other control structures -/
 
-(** A remarkable feature of continuation semantics is that they extend very easily
+/-* A remarkable feature of continuation semantics is that they extend very easily
   to other control structures besides "if-then-else" and "while" loops.
   Consider for instance the "break" construct of C, C++ and Java, which
   immediately terminates the nearest enclosing "while" loop.  Assume we
@@ -600,42 +623,42 @@ Inductive step: com * cont * store -> com * cont * store -> Prop :=
   loop.  Then, the second rule discards the [Kwhile] continuation and
   turns the [BREAK] into a [SKIP], effectively terminating the loop.
   That's all there is to it!
-**)
+*-/
 
-(** *** Exercise (2 stars, recommended) *)
-(** Besides "break", C, C++ and Java also have a "continue" statement
+/-* *** Exercise (2 stars, recommended) -/
+/-* Besides "break", C, C++ and Java also have a "continue" statement
   that terminates the current iteration of the enclosing loop,
   then resumes the loop at its next iteration (instead of stopping
   the loop like "break" does). Give the transition rules
-  for the "continue" statement. *)
+  for the "continue" statement. -/
 
-(** *** Exercise (3 stars, optional) *)
-(** In Java, loops as well as "break" and "continue" statements carry
+/-* *** Exercise (3 stars, optional) -/
+/-* In Java, loops as well as "break" and "continue" statements carry
   an optional label.  "break" without a label exits out of the immediately
   enclosing loop, but "break lbl" exits out of the first enclosing loop
   that carries the label "lbl".  Similarly for "continue".
-  Give the transition rules for "break lbl" and "continue lbl". *)
+  Give the transition rules for "break lbl" and "continue lbl". -/
 
-(** *** Relating the continuation semantics and the big-step semantics *)
+/-* *** Relating the continuation semantics and the big-step semantics -/
 
-(** *** Exercise (2 stars, optional) *)
-(** Show that a big-step execution give rise to a sequence of steps to [SKIP].
-  You can adapt the proof of theorem [cexec_to_reds] with minor changes. *)
+/-* *** Exercise (2 stars, optional) -/
+/-* Show that a big-step execution give rise to a sequence of steps to [SKIP].
+  You can adapt the proof of theorem [cexec_to_reds] with minor changes. -/
 
 Theorem cexec_to_steps:
   forall s c s', cexec s c s' -> forall k, star step (c, k, s) (SKIP, k, s').
 Proof.
   induction 1; intros k.
-  (* FILL IN HERE *)
+  /- FILL IN HERE -/
 Abort.
 
-(** *** Exercise (3 stars, optional) *)
-(** Show the converse result: a sequence of steps to [(SKIP, Kstop)] corresponds
+/-* *** Exercise (3 stars, optional) -/
+/-* Show the converse result: a sequence of steps to [(SKIP, Kstop)] corresponds
   to a big-step execution.  You need a lemma similar to [red_append_cexec],
-  but also a notion of big-step execution of a continuation. *)
+  but also a notion of big-step execution of a continuation. -/
 
 Theorem steps_to_cexec:
   forall c s s', star step (c, Kstop, s) (SKIP, Kstop, s') -> cexec s c s'.
 Proof.
-  (* FILL IN HERE *)
+  /- FILL IN HERE -/
 Abort.
