_notes/Languages/lean/myproject/Myproject.lean
@@ -1,2 +1,14 @@
 import Std.Data.List.Basic
+import Mathlib.Tactic.LibrarySearch
+import Mathlib.Tactic.Linarith
+
+theorem foo : 1 = 1 := by
+  -- library_search
+  exact _root_.trans rfl rfl
+#check _root_.trans
+
+theorem bar : x <= 7 + 3*x := by
+  linarith
+
+#print bar
 def hello := "world"
