_notes/Languages/scheme-racket-lisp.md
@@ -11,6 +11,7 @@ title: Scheme Racket Lisp
 - [Racket](#racket)
     - [Rosette](#rosette)
 - [Common Lisp](#common-lisp)
+  - [ACL2](#acl2)
 - [Compilation](#compilation)
     - [Gambit compiling to javascript](#gambit-compiling-to-javascript)
 - [Misc](#misc)
@@ -134,6 +135,13 @@ SLIME
 [coalton](https://github.com/coalton-lang/coalton)
 
 [alive vscode extension](https://github.com/nobody-famous/alive)
+
+## ACL2
+The main theorem prover associated with common lisp. It is a granddaddy of a lot of other systems
+
+
+
+
 # Compilation
 [http://home.pipeline.com/~hbaker1/CheneyMTA.html](http://home.pipeline.com/~hbaker1/CheneyMTA.html)
 
